cleanup

fmap_functions.thy
@@ -3,12 +3,27 @@ theory fmap_functions
     "~~/src/HOL/Library/Finite_Map"
 begin
 
+section {* Finite maps *}
+
+text {* To keep out model executable, we use finite maps.
+In this theory, we extend the standard library with additional syntax and functions. *}
+
 abbreviation lookupsyntax ("_ .[_]"[25,25]25) where
 "m.[x] \<equiv> fmlookup m x"
 
 abbreviation lookupsyntax2 ("_ ![_]"[25,25]25) where
 "m![x] \<equiv> the (fmlookup m x)"
 
+definition fmap_entries :: "('k, 'v) fmap \<Rightarrow> ('k\<times>'v) set" where
+"fmap_entries m \<equiv> (\<lambda>k. (k, m![k])) ` fmdom' m" 
 
+
+lemma fmap_entries_forall[code_abbrev]: "fmpred P m \<longleftrightarrow> (\<forall>(k,v)\<in>fmap_entries m. P k v)"
+  apply (auto simp add: fmap_entries_def)
+  apply (meson fmdom'_notI fmpredD option.exhaust_sel)
+  by (metis fmdom'I fmpredI option.sel)
+
+lemma fmap_entries_exists[code_abbrev]: "(\<not>fmpred (\<lambda>k v. \<not>P k v) m) \<longleftrightarrow> (\<exists>(k,v)\<in>fmap_entries m. P k v)"
+  by (subst fmap_entries_forall, auto)
 
 end
