ref_crdt.thy
@@ -3,90 +3,13 @@ theory ref_crdt
    "sorted_list"
    fmap_functions
 system_model
+standard_crdts
     "~~/src/HOL/Library/Finite_Map"
     "~~/src/HOL/Library/Open_State_Syntax"
     "~~/src/HOL/Library/Code_Target_Numeral"
 begin
 
 
-section {* System model *}
-
-datatype event = D_event (event_number:int)
-datatype inref = D_inref (inref_number:int)
-datatype ref = D_ref (ref_number:int)
-datatype antidoteKey =  D_antidoteKey int | NullKey
-
-instantiation event :: linorder begin
-definition "less_eq_event x y \<equiv> event_number x \<le> event_number y"
-definition "less_event x y \<equiv> event_number x < event_number y"
-instance by (standard, auto simp add: less_eq_event_def less_event_def event.expand)
-end
-
-instantiation inref :: linorder begin
-definition "less_eq_inref x y \<equiv> inref_number x \<le> inref_number y"
-definition "less_inref x y \<equiv> inref_number x < inref_number y"
-instance by (standard, auto simp add: less_eq_inref_def less_inref_def inref.expand)
-end
-
-instantiation ref :: linorder begin
-definition "less_eq_ref x y \<equiv> ref_number x \<le> ref_number y"
-definition "less_ref x y \<equiv> ref_number x < ref_number y"
-instance by (standard, auto simp add: less_eq_ref_def less_ref_def ref.expand)
-end
-
-instantiation antidoteKey :: linorder begin
-definition "less_antidoteKey1 x y \<equiv> case x of 
-  NullKey \<Rightarrow> y \<noteq> NullKey
-| D_antidoteKey i \<Rightarrow> (case y of
-     NullKey \<Rightarrow> False
-   | D_antidoteKey j \<Rightarrow> i < j)
-"
-definition "less_antidoteKey x y \<equiv> less_antidoteKey1 x y"
-definition "less_eq_antidoteKey x y \<equiv> x=y \<or> less_antidoteKey1 x y "
-instance 
-  apply standard
-      apply (auto simp add: less_antidoteKey_def less_eq_antidoteKey_def less_antidoteKey1_def  split: antidoteKey.splits ref.splits inref.splits)
-  done
-end
-
-
-
-instantiation prod :: (linorder,linorder) linorder begin
-definition "less_prod x y \<equiv> fst x < fst y \<or> fst x = fst y \<and> snd x < snd y"
-definition "less_eq_prod x y \<equiv> fst x < fst y \<or> fst x = fst y \<and> snd x \<le> snd y"
-instance 
-  apply standard
-      apply (auto simp add: less_prod_def less_eq_prod_def)
-  done
-end
-
-instantiation option :: (linorder) linorder begin
-definition "less_option x y \<equiv> case x of None \<Rightarrow> y\<noteq>None | Some x' \<Rightarrow> (case y of None \<Rightarrow> False | Some y' \<Rightarrow> x' < y')"
-definition "less_eq_option x y \<equiv> case x of None \<Rightarrow> True | Some x' \<Rightarrow> (case y of None \<Rightarrow> False | Some y' \<Rightarrow> x' \<le> y')"
-instance 
-  apply standard
-      apply (auto simp add: less_option_def less_eq_option_def split: option.splits)
-  done
-end
-
-definition fmap_entries :: "('k, 'v) fmap \<Rightarrow> ('k\<times>'v) set" where
-"fmap_entries m \<equiv> (\<lambda>k. (k, m![k])) ` fmdom' m" 
-
-
-lemma fmap_entries_forall[code_abbrev]: "fmpred P m \<longleftrightarrow> (\<forall>(k,v)\<in>fmap_entries m. P k v)"
-  apply (auto simp add: fmap_entries_def)
-  apply (meson fmdom'_notI fmpredD option.exhaust_sel)
-  by (metis fmdom'I fmpredI option.sel)
-
-lemma fmap_entries_exists[code_abbrev]: "(\<not>fmpred (\<lambda>k v. \<not>P k v) m) \<longleftrightarrow> (\<exists>(k,v)\<in>fmap_entries m. P k v)"
-  by (subst fmap_entries_forall, auto)
-
-
-definition orElse (infixr "orElse" 25) where
-"x orElse y \<equiv> (case x of Some a \<Rightarrow> a | None \<Rightarrow> y)"
-
-(* using event-IDs to model unique identifiers *)
-type_synonym uid = event
 
 datatype operation = 
     init ref inref
@@ -102,22 +25,12 @@ datatype operation_effector =
   | effector_inref_rev_refs_add inref ref uid
   | effector_inref_rev_refs_rem inref ref uid
   | effector_ref_dest_keys_assign ref "inref option" uid "uid set"
-    (*effector_init ref inref uid (f_dest_uids:"uid set")
-  | effector_assign ref ref
-  | effector_deref ref
-  | effector_may_delete inref "ref list"
-  | effector_reset_inref inref
-  | effector_reset_ref ref
-*)
 
 datatype operation_result =
     deref_result "antidoteKey option"
   | no_result
   | may_delete_result bool
 
-type_synonym 'a mv_register_state = "('a \<times> uid) set"
-  
-type_synonym 'a two_phase_set_state = "'a set \<times> 'a set"  
 
 record ref_state =
   object_key :: "antidoteKey"
@@ -132,231 +45,6 @@ record state =
   state_refs :: "(ref, ref_state) fmap"
   state_inrefs :: "(inref, inref_state) fmap"
 
-datatype snapshot = Snapshot (snapshot_map: "(event,nat) fmap")
-
-abbreviation "snapshot_events s \<equiv> fmdom' (snapshot_map s)"
-abbreviation "snapshot_entries s \<equiv> fmap_entries (snapshot_map s)"
-abbreviation "snapshot_num s e \<equiv> case (snapshot_map s).[e] of Some n \<Rightarrow> Suc n | None \<Rightarrow> 0"
-definition includedIn where
-"includedIn e n snapshot \<equiv> n < snapshot_num snapshot e"
-
-instantiation snapshot :: preorder begin
-
-
-definition less_eq_snapshot  :: "snapshot \<Rightarrow> snapshot \<Rightarrow> bool"  where
-"less_eq_snapshot x y \<equiv> \<forall>(e,n)\<in>snapshot_entries x. Suc n \<le> snapshot_num y e"
-definition "less_snapshot x y \<equiv> (\<forall>(e,n)\<in>snapshot_entries x. Suc n \<le> snapshot_num y e) \<and> (\<exists>(e,n)\<in>snapshot_entries y. n \<ge> snapshot_num x e )"
-
-
-instance
-proof 
-  fix x y z :: snapshot
-  obtain x' y' z' where [simp]: "x = Snapshot x'" and [simp]: "y = Snapshot y'" and [simp]: "z = Snapshot z'"
-    by (metis snapshot.collapse)
-
-  show "(x < y) = (x \<le> y \<and> \<not> y \<le> x)"
-    apply (auto simp add: less_eq_snapshot_def less_snapshot_def  orElse_def fmap_entries_def fmlookup_dom'_iff  split: option.splits)
-    using fmdom'I apply force
-    by (metis fmdom'I not_less_eq_eq option.sel)
-
-
-  show "x \<le> x"
-    by (auto simp add: less_eq_snapshot_def fmap_entries_def orElse_def fmdom'_notI fmlookup_dom'_iff split: option.splits)
-
-  show "\<lbrakk>x \<le> y; y \<le> z\<rbrakk> \<Longrightarrow> x \<le> z"
-    apply (auto simp add: less_eq_snapshot_def fmap_entries_def orElse_def fmdom'_notI split: option.splits)
-    apply (meson fmdom'I)
-    by fastforce
-    
-qed
-
-end
-
-
-record eventInfo =
-  event_operation :: "operation"
-  event_result :: operation_result
-  event_effectors :: "operation_effector list"
-  event_executionOrder :: "event list"
-  event_state_pre :: state (* state before executing the event *)
-  event_state_post :: state (* state after executing the event *)
-  event_snapshot :: snapshot  (* events that happened before and how many of their effectors are included in the snapshot *)
-                          
-record execution =
-  events :: "(event, eventInfo) fmap"
-  
-
-
-
-abbreviation "events' E \<equiv> fmap_entries (events E)"
-abbreviation "eventsIds E \<equiv> fmdom' (events E)"
-
-definition happensBeforeP :: "event \<Rightarrow> event \<Rightarrow> execution \<Rightarrow> bool" ("_ happened before _ in _" [25,25,25]25) where
-"x happened before y in E \<equiv> 
-   case (events E).[y] of 
-     None \<Rightarrow> False 
-   | Some yInfo \<Rightarrow> (
-      case (events E).[x] of
-       None \<Rightarrow> False 
-     | Some xInfo \<Rightarrow> includedIn x (length (event_effectors xInfo)) (event_snapshot yInfo)
-  ) "
-
-definition happensBefore :: "execution \<Rightarrow> event rel"  where
-"happensBefore E \<equiv> {(x,y). x happened before y in E}"
-
-
-lemma happensBefore_code[code]:
-"happensBefore E = \<Union> ((\<lambda>(e,eInfo). (Set.filter (\<lambda>e'. e' happened before e in E) (snapshot_events (event_snapshot eInfo))) \<times> {e} )  ` fmap_entries (events E))"
-  apply (auto simp add: happensBefore_def happensBeforeP_def  split: option.splits)
-  apply (rule_tac x="(b,y)" in bexI)
-  apply (auto simp add: fmap_entries_def fmdom'I image_iff)
-  using fmlookup_dom'_iff includedIn_def by fastforce
-
-
-lemma in_happensBefore_code[code_abbrev]: "(x happened before y in E) \<longleftrightarrow> (x,y)\<in>happensBefore E"
-  by (auto simp add: happensBefore_def happensBeforeP_def fmdom'I split: option.splits)
-
-export_code happensBefore in Haskell
-
-
-definition "foo x y E \<equiv> \<forall>(e,ei)\<in>fmap_entries(events E). True" 
-
-export_code foo in Haskell
-
-type_synonym generator_function = "(operation \<Rightarrow> uid \<Rightarrow> state \<Rightarrow> operation_result \<times> (operation_effector list))"
-type_synonym effector_function = "(operation_effector \<Rightarrow> state \<Rightarrow> state)"
-
-definition compose_forward (infixl "|>" 25) where
-"x |> f \<equiv> f x"
-
-value "(1::int) |> op+ 1 |> op* 2"
-
-definition "wf_causallyConsistent E \<equiv> 
-\<forall>(e,eInfo)\<in>events' E. \<forall>(e',i)\<in>snapshot_entries(event_snapshot eInfo). 
-  case (events E).[e'] of
-      None \<Rightarrow> False
-    | Some eInfo' \<Rightarrow> event_snapshot eInfo' \<le> event_snapshot eInfo
-"
-
-definition "partial_order_on2 S R \<equiv> 
-fst ` R \<subseteq>  S
-\<and> snd ` R \<subseteq>  S
-\<and> (\<forall>x\<in>S. (x,x)\<in>R)
-\<and> R\<^sup>+ \<subseteq> R
-\<and> (\<forall>x\<in>S. \<forall>y\<in>S. (x,y)\<in>R \<and> (y,x)\<in>R \<longrightarrow> x = y)
-"
-
-lemma partial_order_on2_eq: "partial_order_on2 S R = partial_order_on S R"
-  apply (auto simp add: partial_order_on2_def partial_order_on_def preorder_on_def refl_on_domain refl_onD antisymD)
-    apply (auto simp add: refl_on_def)[1]
-   apply (auto simp add: trans_def)[1]
-  apply (auto simp add: antisym_def)[1]
-  by (metis fst_conv image_subset_iff)
-
-
-export_code wf_causallyConsistent in Haskell
-
-
-
-definition wf_generator :: "execution \<Rightarrow> generator_function \<Rightarrow> bool" where
-"wf_generator execution gen \<equiv>
-events execution |> fmpred (\<lambda>e eInfo.
-  gen (event_operation eInfo)  e (event_state_pre eInfo) = (event_result eInfo, event_effectors eInfo)) 
-"
-
-
-
-definition executeEffectors :: "operation_effector list \<Rightarrow> state \<Rightarrow> effector_function \<Rightarrow> state" where
-"executeEffectors effectors initial eff \<equiv> foldl (\<lambda>s e. eff e s) initial effectors "
-
-definition sorted_partial :: "'a list \<Rightarrow> 'a rel \<Rightarrow> bool" where
-"sorted_partial list rel \<equiv> (\<forall>j<length list. \<forall>i<j. (list!j, list!i)\<notin>rel)"
-
-
-definition
-"valid_event_sequence eventList eventSet hb \<equiv> 
-set eventList = eventSet \<and> distinct eventList \<and> sorted_partial eventList hb"
-
-
-definition "previous_events hb e \<equiv> fst ` Set.filter (\<lambda>(x,y). y = e \<and> x\<noteq>e) hb"  (* or {e'.  e'\<noteq>e \<and> (e',e)\<in>hb}*)
-definition "downwards_closure S E \<equiv> S \<union>  (\<Union>e\<in>S. case (events E).[e] of None \<Rightarrow> {} | Some info \<Rightarrow> snapshot_events (event_snapshot info))"
-definition "parallel_closure S A hb \<equiv> Set.filter (\<lambda>x. x\<in>S \<or> (\<exists>y\<in>S. (y,x)\<notin>hb)) A"
-
-value "parallel_closure {1,2::int} {1,2,3,4,5} ({(2,3), (2,4), (1,4), (1,1), (2,2), (3,3), (4,4), (5,5)}\<^sup>+)"
-
-value "parallel_closure {} {1::int,2,3,4,5} ({(2,3), (1,4), (1,1), (2,2), (3,3), (4,4), (5,5)}\<^sup>+)"
-
-
-export_code previous_events in Haskell
-
-definition 
-"wf_correct_execution_lists execution \<equiv> 
-events execution |> fmpred (\<lambda>e eInfo. valid_event_sequence (event_executionOrder eInfo) (previous_events (happensBefore execution) e) (happensBefore execution))
-"
-
-export_code wf_correct_execution_lists
-
-find_consts "('a \<Rightarrow> 'b list) => 'a list => 'b list"
-
-definition wf_effector :: "execution \<Rightarrow> state \<Rightarrow> effector_function \<Rightarrow> bool" where
-"wf_effector execution initS eff \<equiv>
-events execution |> fmpred (\<lambda>e eInfo. 
-  let effectors = event_executionOrder eInfo |> List.maps (\<lambda>e'. 
-      case (events execution).[e'] of Some eInfo' \<Rightarrow> take (snapshot_num (event_snapshot eInfo) e') (event_effectors eInfo') | None \<Rightarrow> [])
-  in
-  event_state_pre eInfo = executeEffectors effectors initS eff
-  \<and> event_state_post eInfo = executeEffectors (event_effectors eInfo) (event_state_pre eInfo) eff)
-"
-
-definition 
-"wf_localPreconditions execution localPred \<equiv>
-events execution |> fmpred (\<lambda>e eInfo.  localPred (event_operation eInfo) (event_state_pre eInfo))
-"
-
-
-definition 
-"closed_concurrent e hb E \<equiv> \<forall>e1\<in>E. e1\<noteq>e \<and> (e1, e)\<in>hb \<longrightarrow> (\<forall>e2\<in>E.(e1,e2)\<notin>hb \<and> (e2,e1)\<notin>hb \<longrightarrow> (e2, e)\<in>hb)"
-
-text {* Define that event e has received all effectors from its dependencies. *}
-definition 
-"fullSnapshot e E \<equiv> 
-  case (events E).[e] of 
-      None \<Rightarrow> False
-    | Some info \<Rightarrow> (\<forall>(e',n)\<in>snapshot_entries (event_snapshot info). 
-        case (events E).[e'] of
-            None \<Rightarrow> False
-          | Some info' \<Rightarrow> n \<ge> length (event_effectors info'))"
-
-definition
-"stable e E \<equiv> closed_concurrent e (happensBefore E) (fmdom' (events E))
-            \<and> fullSnapshot e E  "
-
-
-definition 
-"wf_stablePreconditions execution pred \<equiv>
-events execution |> fmpred (\<lambda>e eInfo. 
-    case pred (event_operation eInfo) of 
-       None \<Rightarrow> True
-     | Some cond \<Rightarrow> 
-        stable e execution
-      \<and> cond (event_state_pre eInfo))
-"
-
-export_code closed_concurrent in Haskell
-export_code wf_stablePreconditions in Haskell
-
-
-definition wellFormed :: "execution \<Rightarrow> state \<Rightarrow> generator_function \<Rightarrow> effector_function \<Rightarrow> (operation \<Rightarrow> state \<Rightarrow> bool) \<Rightarrow> (operation \<rightharpoonup> state \<Rightarrow> bool) \<Rightarrow> bool"
-where
-"wellFormed execution initS gen eff localPre pre \<equiv>
-    wf_causallyConsistent execution 
-  \<and> wf_correct_execution_lists execution
-  \<and> wf_generator execution gen
-  \<and> wf_effector execution initS eff
-  \<and> wf_localPreconditions execution localPre
-  \<and> wf_stablePreconditions execution pre"
-
-
 
 definition initialState :: state where 
 "initialState \<equiv> \<lparr>
@@ -364,19 +52,10 @@ definition initialState :: state where
   state_inrefs = fmempty
  \<rparr>"                                              
 
-
-definition run :: "state \<Rightarrow> (state \<Rightarrow> state) list \<Rightarrow> state"  where
-"run start actions \<equiv> foldl (\<lambda>s f. f s) start actions"
-
-fun two_phase_set_add where 
-"two_phase_set_add (A,R) (x, uid) = (insert (x,uid) A, R)"
-
-fun two_phase_set_remove where 
-"two_phase_set_remove (A,R) (x, uid) = (A,insert (x,uid) R)"
-
-term fmlookup
-find_consts "('a, 'b) fmap \<Rightarrow> 'a \<Rightarrow> 'b \<Rightarrow> 'b" 
-
+type_synonym generator_function = "(operation \<Rightarrow> uid \<Rightarrow> state \<Rightarrow> operation_result \<times> (operation_effector list))"
+type_synonym effector_function = "(operation_effector \<Rightarrow> state \<Rightarrow> state)"
+type_synonym execution' = "(operation, operation_result, operation_effector, state) execution"
+type_synonym eventInfo' = "(operation, operation_result, operation_effector, state) eventInfo"
 
 definition return :: "'a \<Rightarrow> operation_effector list \<Rightarrow> ('a \<times> operation_effector list)" where
 "return r l = (r,l)"
@@ -435,20 +114,6 @@ definition s_update_inref :: "inref \<Rightarrow> (inref_state \<Rightarrow> inr
 definition s_update_ref :: "ref \<Rightarrow> (ref_state \<Rightarrow> ref_state) \<Rightarrow> state \<Rightarrow> state" where
 "s_update_ref ref f S \<equiv> S\<lparr>state_refs := fmupd ref (f (ref_state S ref)) (state_refs S)\<rparr>"
 
-definition mv_reg_getall :: "'a mv_register_state \<Rightarrow> 'a set" where
-"mv_reg_getall s = (fst ` s)"
-
-definition mv_reg_get1 :: "'a::linorder mv_register_state \<Rightarrow> 'a \<Rightarrow> 'a" where
-"mv_reg_get1 s d \<equiv> let all = mv_reg_getall s in if all = {} then d else Max (mv_reg_getall s)"
-
-definition mv_reg_get1' where
-"mv_reg_get1' s \<equiv> mv_reg_get1 s None"
-
-definition mv_reg_count :: "'a mv_register_state \<Rightarrow> nat" where
-"mv_reg_count s = card (mv_reg_getall s)"
-
-definition two_phase_set_get :: "'a two_phase_set_state \<Rightarrow> 'a set" where
-"two_phase_set_get s \<equiv> fst s - snd s"
 
 definition may_delete_check :: "state \<Rightarrow> inref \<Rightarrow> ref set \<Rightarrow> bool" where
 "may_delete_check state inref last_refs \<equiv> 
@@ -621,7 +286,7 @@ find_consts "('k, 'v) fmap"
 
 definition "numberEffectors E e \<equiv> e |> fmlookup (events E) |> the |> event_effectors |> length"
 
-definition execution_addStep :: "int \<Rightarrow> operation \<Rightarrow> (event,nat) fmap \<Rightarrow> execution \<Rightarrow> execution" where
+definition execution_addStep :: "int \<Rightarrow> operation \<Rightarrow> (event,nat) fmap \<Rightarrow> execution' \<Rightarrow> execution'" where
 "execution_addStep eId opr preEventsN E \<equiv> 
 let
    e = D_event eId;
@@ -672,25 +337,25 @@ record trace_event =
   t_operation :: operation
   t_deps :: "(event,nat) fmap"
 
-definition execution_run :: "trace_event list \<Rightarrow> execution" where
+definition execution_run :: "trace_event list \<Rightarrow> execution'" where
 "execution_run ops \<equiv> snd (fold (\<lambda>e (n,E). (n+1, execution_addStep n (t_operation e) (t_deps e) E)) ops (0, emptyExecution))"
 
-definition forallEvents :: "execution \<Rightarrow> (event \<Rightarrow> eventInfo \<Rightarrow> bool) \<Rightarrow> bool" where
+definition forallEvents :: "execution' \<Rightarrow> (event \<Rightarrow> eventInfo' \<Rightarrow> bool) \<Rightarrow> bool" where
 "forallEvents E P \<equiv> events E |> fmpred P"
 
-definition forallStates :: "execution \<Rightarrow> (state \<Rightarrow> bool) \<Rightarrow> bool" where
+definition forallStates :: "execution' \<Rightarrow> (state \<Rightarrow> bool) \<Rightarrow> bool" where
 "forallStates E P \<equiv> forallEvents E (\<lambda>e eInfo. P (event_state_pre eInfo) \<and> P (event_state_post eInfo))"
 
 
 subsection {* Invariants *}
 
 (* if ref exists, inref exists *)
-definition invariant1 :: "execution \<Rightarrow> bool" where
+definition invariant1 :: "execution' \<Rightarrow> bool" where
 "invariant1 E \<equiv> forallStates E (\<lambda>s. state_refs s |> fmpred (\<lambda>r rState. \<forall>(k,u)\<in>dest_keys rState. case k of None \<Rightarrow> True | Some inref \<Rightarrow> 
    (case (state_inrefs s).[inref] of None \<Rightarrow> False | Some inrefState \<Rightarrow> (r,u) \<in> two_phase_set_get (rev_refs inrefState) )))"
 
 (* once an inref is unreachable, it remains unreachable *)
-definition invariant2 :: "execution \<Rightarrow> bool" where
+definition invariant2 :: "execution' \<Rightarrow> bool" where
 "invariant2 E \<equiv> 
 (\<forall>(e,eInfo)\<in>events' E. 
   \<forall>(inref,inrefState)\<in>fmap_entries (state_inrefs (event_state_pre eInfo)). 
@@ -705,7 +370,7 @@ definition invariant2 :: "execution \<Rightarrow> bool" where
 (* if there is a reverse reference, then there is also a forward reference
 (only true, if using transactional semantics )
  *)
-definition invariant3 :: "execution \<Rightarrow> bool" where
+definition invariant3 :: "execution' \<Rightarrow> bool" where
 "invariant3 E \<equiv> 
 forallStates E (\<lambda>S. 
   \<forall>(inref,inrefState)\<in>fmap_entries (state_inrefs S).  
@@ -717,7 +382,7 @@ forallStates E (\<lambda>S.
 "
 
 (* some simple postconditions for operations*)
-definition invariant4 :: "execution \<Rightarrow> bool" where
+definition invariant4 :: "execution' \<Rightarrow> bool" where
 "invariant4 E \<equiv> 
 \<forall>(e,eInfo)\<in>events' E. 
 case event_operation eInfo of
@@ -731,7 +396,7 @@ case event_operation eInfo of
 
 (* finally: if there is a reverse reference, then there is also a forward reference
  *)
-definition invariant5 :: "execution \<Rightarrow> bool" where
+definition invariant5 :: "execution' \<Rightarrow> bool" where
 "invariant5 E \<equiv>   
 let 
 execution_order = sorted_list_of_set2 (fmdom' (events E));
