system_model.thy
@@ -1,191 +1,40 @@
+(*<*)
 theory system_model
-imports fmap_functions
+  imports fmap_functions
+    system_model_types
+    standard_crdts
+    snapshot
 begin 
-
+(*>*)
 
 section {* System model *}
 
-datatype event = D_event (event_number:int)
-datatype inref = D_inref (inref_number:int)
-datatype ref = D_ref (ref_number:int)
-datatype antidoteKey =  D_antidoteKey int | NullKey
+text {*
+We parameterize our Model based on four type parameters:
 
-instantiation event :: linorder begin
-definition "less_eq_event x y \<equiv> event_number x \<le> event_number y"
-definition "less_event x y \<equiv> event_number x < event_number y"
-instance by (standard, auto simp add: less_eq_event_def less_event_def event.expand)
-end
+ - The operation type describes which operations can be executed via the API.
+ - The operation-result type determines what are possible results of operations.
+ - The operation-effector type describes, which messages can be sent to other replicas as effectors.
+ - The state type describes the state at each replica.
 
-instantiation inref :: linorder begin
-definition "less_eq_inref x y \<equiv> inref_number x \<le> inref_number y"
-definition "less_inref x y \<equiv> inref_number x < inref_number y"
-instance by (standard, auto simp add: less_eq_inref_def less_inref_def inref.expand)
-end
+*}
 
-instantiation ref :: linorder begin
-definition "less_eq_ref x y \<equiv> ref_number x \<le> ref_number y"
-definition "less_ref x y \<equiv> ref_number x < ref_number y"
-instance by (standard, auto simp add: less_eq_ref_def less_ref_def ref.expand)
-end
-
-instantiation antidoteKey :: linorder begin
-definition "less_antidoteKey1 x y \<equiv> case x of 
-  NullKey \<Rightarrow> y \<noteq> NullKey
-| D_antidoteKey i \<Rightarrow> (case y of
-     NullKey \<Rightarrow> False
-   | D_antidoteKey j \<Rightarrow> i < j)
-"
-definition "less_antidoteKey x y \<equiv> less_antidoteKey1 x y"
-definition "less_eq_antidoteKey x y \<equiv> x=y \<or> less_antidoteKey1 x y "
-instance 
-  apply standard
-      apply (auto simp add: less_antidoteKey_def less_eq_antidoteKey_def less_antidoteKey1_def  split: antidoteKey.splits ref.splits inref.splits)
-  done
-end
-
-
-
-instantiation prod :: (linorder,linorder) linorder begin
-definition "less_prod x y \<equiv> fst x < fst y \<or> fst x = fst y \<and> snd x < snd y"
-definition "less_eq_prod x y \<equiv> fst x < fst y \<or> fst x = fst y \<and> snd x \<le> snd y"
-instance 
-  apply standard
-      apply (auto simp add: less_prod_def less_eq_prod_def)
-  done
-end
-
-instantiation option :: (linorder) linorder begin
-definition "less_option x y \<equiv> case x of None \<Rightarrow> y\<noteq>None | Some x' \<Rightarrow> (case y of None \<Rightarrow> False | Some y' \<Rightarrow> x' < y')"
-definition "less_eq_option x y \<equiv> case x of None \<Rightarrow> True | Some x' \<Rightarrow> (case y of None \<Rightarrow> False | Some y' \<Rightarrow> x' \<le> y')"
-instance 
-  apply standard
-      apply (auto simp add: less_option_def less_eq_option_def split: option.splits)
-  done
-end
-
-definition fmap_entries :: "('k, 'v) fmap \<Rightarrow> ('k\<times>'v) set" where
-"fmap_entries m \<equiv> (\<lambda>k. (k, m![k])) ` fmdom' m" 
-
-
-lemma fmap_entries_forall[code_abbrev]: "fmpred P m \<longleftrightarrow> (\<forall>(k,v)\<in>fmap_entries m. P k v)"
-  apply (auto simp add: fmap_entries_def)
-  apply (meson fmdom'_notI fmpredD option.exhaust_sel)
-  by (metis fmdom'I fmpredI option.sel)
-
-lemma fmap_entries_exists[code_abbrev]: "(\<not>fmpred (\<lambda>k v. \<not>P k v) m) \<longleftrightarrow> (\<exists>(k,v)\<in>fmap_entries m. P k v)"
-  by (subst fmap_entries_forall, auto)
-
-
-definition orElse (infixr "orElse" 25) where
-"x orElse y \<equiv> (case x of Some a \<Rightarrow> a | None \<Rightarrow> y)"
-
-(* using event-IDs to model unique identifiers *)
-type_synonym uid = event
-
-datatype operation = 
-    init ref inref
-  | assign ref ref
-  | deref ref
-  | may_delete inref "ref list"
-  | reset_inref inref
-  | reset_ref ref
- (* TODO resolve *)
-
-datatype operation_effector = 
-    effector_inref_inuse_enable inref
-  | effector_inref_rev_refs_add inref ref uid
-  | effector_inref_rev_refs_rem inref ref uid
-  | effector_ref_dest_keys_assign ref "inref option" uid "uid set"
-    (*effector_init ref inref uid (f_dest_uids:"uid set")
-  | effector_assign ref ref
-  | effector_deref ref
-  | effector_may_delete inref "ref list"
-  | effector_reset_inref inref
-  | effector_reset_ref ref
-*)
-
-datatype operation_result =
-    deref_result "antidoteKey option"
-  | no_result
-  | may_delete_result bool
-
-type_synonym 'a mv_register_state = "('a \<times> uid) set"
-  
-type_synonym 'a two_phase_set_state = "'a set \<times> 'a set"  
-
-record ref_state =
-  object_key :: "antidoteKey"
-  dest_keys :: "inref option mv_register_state"
-
-record inref_state =
-  inref_object_key :: "antidoteKey"
-  rev_refs :: "(ref \<times> uid) two_phase_set_state"
-  inUse :: bool
-
-record state =
-  state_refs :: "(ref, ref_state) fmap"
-  state_inrefs :: "(inref, inref_state) fmap"
-
-datatype snapshot = Snapshot (snapshot_map: "(event,nat) fmap")
-
-abbreviation "snapshot_events s \<equiv> fmdom' (snapshot_map s)"
-abbreviation "snapshot_entries s \<equiv> fmap_entries (snapshot_map s)"
-abbreviation "snapshot_num s e \<equiv> case (snapshot_map s).[e] of Some n \<Rightarrow> Suc n | None \<Rightarrow> 0"
-definition includedIn where
-"includedIn e n snapshot \<equiv> n < snapshot_num snapshot e"
-
-instantiation snapshot :: preorder begin
-
-
-definition less_eq_snapshot  :: "snapshot \<Rightarrow> snapshot \<Rightarrow> bool"  where
-"less_eq_snapshot x y \<equiv> \<forall>(e,n)\<in>snapshot_entries x. Suc n \<le> snapshot_num y e"
-definition "less_snapshot x y \<equiv> (\<forall>(e,n)\<in>snapshot_entries x. Suc n \<le> snapshot_num y e) \<and> (\<exists>(e,n)\<in>snapshot_entries y. n \<ge> snapshot_num x e )"
-
-
-instance
-proof 
-  fix x y z :: snapshot
-  obtain x' y' z' where [simp]: "x = Snapshot x'" and [simp]: "y = Snapshot y'" and [simp]: "z = Snapshot z'"
-    by (metis snapshot.collapse)
-
-  show "(x < y) = (x \<le> y \<and> \<not> y \<le> x)"
-    apply (auto simp add: less_eq_snapshot_def less_snapshot_def  orElse_def fmap_entries_def fmlookup_dom'_iff  split: option.splits)
-    using fmdom'I apply force
-    by (metis fmdom'I not_less_eq_eq option.sel)
-
-
-  show "x \<le> x"
-    by (auto simp add: less_eq_snapshot_def fmap_entries_def orElse_def fmdom'_notI fmlookup_dom'_iff split: option.splits)
-
-  show "\<lbrakk>x \<le> y; y \<le> z\<rbrakk> \<Longrightarrow> x \<le> z"
-    apply (auto simp add: less_eq_snapshot_def fmap_entries_def orElse_def fmdom'_notI split: option.splits)
-    apply (meson fmdom'I)
-    by fastforce
-    
-qed
-
-end
-
-
-record eventInfo =
-  event_operation :: "operation"
-  event_result :: operation_result
-  event_effectors :: "operation_effector list"
+record ('operation, 'operation_result, 'operation_effector, 'state) eventInfo =
+  event_operation :: "'operation"
+  event_result :: 'operation_result
+  event_effectors :: "'operation_effector list"
   event_executionOrder :: "event list"
-  event_state_pre :: state (* state before executing the event *)
-  event_state_post :: state (* state after executing the event *)
+  event_state_pre :: 'state (* state before executing the event *)
+  event_state_post :: 'state (* state after executing the event *)
   event_snapshot :: snapshot  (* events that happened before and how many of their effectors are included in the snapshot *)
                           
-record execution =
-  events :: "(event, eventInfo) fmap"
+record ('operation, 'operation_result, 'operation_effector, 'state) execution =
+  events :: "(event, ('operation, 'operation_result, 'operation_effector, 'state) eventInfo) fmap"
   
-
-
-
 abbreviation "events' E \<equiv> fmap_entries (events E)"
 abbreviation "eventsIds E \<equiv> fmdom' (events E)"
 
-definition happensBeforeP :: "event \<Rightarrow> event \<Rightarrow> execution \<Rightarrow> bool" ("_ happened before _ in _" [25,25,25]25) where
+definition happensBeforeP :: "event \<Rightarrow> event \<Rightarrow> ('operation, 'operation_result, 'operation_effector, 'state) execution \<Rightarrow> bool" ("_ happened before _ in _" [25,25,25]25) where
 "x happened before y in E \<equiv> 
    case (events E).[y] of 
      None \<Rightarrow> False 
@@ -195,7 +44,7 @@ definition happensBeforeP :: "event \<Rightarrow> event \<Rightarrow> execution 
      | Some xInfo \<Rightarrow> includedIn x (length (event_effectors xInfo)) (event_snapshot yInfo)
   ) "
 
-definition happensBefore :: "execution \<Rightarrow> event rel"  where
+definition happensBefore :: "('operation, 'operation_result, 'operation_effector, 'state) execution \<Rightarrow> event rel"  where
 "happensBefore E \<equiv> {(x,y). x happened before y in E}"
 
 
@@ -217,13 +66,10 @@ definition "foo x y E \<equiv> \<forall>(e,ei)\<in>fmap_entries(events E). True"
 
 export_code foo in Haskell
 
-type_synonym generator_function = "(operation \<Rightarrow> uid \<Rightarrow> state \<Rightarrow> operation_result \<times> (operation_effector list))"
-type_synonym effector_function = "(operation_effector \<Rightarrow> state \<Rightarrow> state)"
+type_synonym ('operation, 'operation_result, 'operation_effector, 'state) generator_function = "('operation \<Rightarrow> uid \<Rightarrow> 'state \<Rightarrow> 'operation_result \<times> ('operation_effector list))"
+type_synonym ('operation_effector, 'state) effector_function = "('operation_effector \<Rightarrow> 'state \<Rightarrow> 'state)"
 
-definition compose_forward (infixl "|>" 25) where
-"x |> f \<equiv> f x"
 
-value "(1::int) |> op+ 1 |> op* 2"
 
 definition "wf_causallyConsistent E \<equiv> 
 \<forall>(e,eInfo)\<in>events' E. \<forall>(e',i)\<in>snapshot_entries(event_snapshot eInfo). 
@@ -232,27 +78,10 @@ definition "wf_causallyConsistent E \<equiv>
     | Some eInfo' \<Rightarrow> event_snapshot eInfo' \<le> event_snapshot eInfo
 "
 
-definition "partial_order_on2 S R \<equiv> 
-fst ` R \<subseteq>  S
-\<and> snd ` R \<subseteq>  S
-\<and> (\<forall>x\<in>S. (x,x)\<in>R)
-\<and> R\<^sup>+ \<subseteq> R
-\<and> (\<forall>x\<in>S. \<forall>y\<in>S. (x,y)\<in>R \<and> (y,x)\<in>R \<longrightarrow> x = y)
-"
-
-lemma partial_order_on2_eq: "partial_order_on2 S R = partial_order_on S R"
-  apply (auto simp add: partial_order_on2_def partial_order_on_def preorder_on_def refl_on_domain refl_onD antisymD)
-    apply (auto simp add: refl_on_def)[1]
-   apply (auto simp add: trans_def)[1]
-  apply (auto simp add: antisym_def)[1]
-  by (metis fst_conv image_subset_iff)
-
-
-export_code wf_causallyConsistent in Haskell
 
 
 
-definition wf_generator :: "execution \<Rightarrow> generator_function \<Rightarrow> bool" where
+definition wf_generator :: "('operation, 'operation_result, 'operation_effector, 'state) execution \<Rightarrow> ('operation, 'operation_result, 'operation_effector, 'state)generator_function \<Rightarrow> bool" where
 "wf_generator execution gen \<equiv>
 events execution |> fmpred (\<lambda>e eInfo.
   gen (event_operation eInfo)  e (event_state_pre eInfo) = (event_result eInfo, event_effectors eInfo)) 
@@ -260,7 +89,7 @@ events execution |> fmpred (\<lambda>e eInfo.
 
 
 
-definition executeEffectors :: "operation_effector list \<Rightarrow> state \<Rightarrow> effector_function \<Rightarrow> state" where
+definition executeEffectors :: "'operation_effector list \<Rightarrow> 'state \<Rightarrow> ('operation_effector, 'state) effector_function \<Rightarrow> 'state" where
 "executeEffectors effectors initial eff \<equiv> foldl (\<lambda>s e. eff e s) initial effectors "
 
 definition sorted_partial :: "'a list \<Rightarrow> 'a rel \<Rightarrow> bool" where
@@ -292,7 +121,7 @@ export_code wf_correct_execution_lists
 
 find_consts "('a \<Rightarrow> 'b list) => 'a list => 'b list"
 
-definition wf_effector :: "execution \<Rightarrow> state \<Rightarrow> effector_function \<Rightarrow> bool" where
+definition wf_effector :: "('operation, 'operation_result, 'operation_effector, 'state)execution \<Rightarrow> 'state \<Rightarrow> ('operation_effector, 'state) effector_function \<Rightarrow> bool" where
 "wf_effector execution initS eff \<equiv>
 events execution |> fmpred (\<lambda>e eInfo. 
   let effectors = event_executionOrder eInfo |> List.maps (\<lambda>e'. 
@@ -340,7 +169,7 @@ export_code closed_concurrent in Haskell
 export_code wf_stablePreconditions in Haskell
 
 
-definition wellFormed :: "execution \<Rightarrow> state \<Rightarrow> generator_function \<Rightarrow> effector_function \<Rightarrow> (operation \<Rightarrow> state \<Rightarrow> bool) \<Rightarrow> (operation \<rightharpoonup> state \<Rightarrow> bool) \<Rightarrow> bool"
+definition wellFormed :: "('operation, 'operation_result, 'operation_effector, 'state) execution \<Rightarrow> 'state \<Rightarrow> ('operation, 'operation_result, 'operation_effector, 'state) generator_function \<Rightarrow> ( 'operation_effector, 'state) effector_function \<Rightarrow> ('operation \<Rightarrow> 'state \<Rightarrow> bool) \<Rightarrow> ('operation \<rightharpoonup> 'state \<Rightarrow> bool) \<Rightarrow> bool"
 where
 "wellFormed execution initS gen eff localPre pre \<equiv>
     wf_causallyConsistent execution 
@@ -352,11 +181,6 @@ where
 
 
 
-definition initialState :: state where 
-"initialState \<equiv> \<lparr>
-  state_refs = fmempty,
-  state_inrefs = fmempty
- \<rparr>"                                              
 
 
 end
