snapshot.thy
@@ -1,0 +1,53 @@
+theory snapshot
+  imports Main 
+    system_model_types
+    fmap_functions
+sugar
+begin
+
+
+section {* Snapshots *}
+
+
+
+datatype snapshot = Snapshot (snapshot_map: "(event,nat) fmap")
+
+abbreviation "snapshot_events s \<equiv> fmdom' (snapshot_map s)"
+abbreviation "snapshot_entries s \<equiv> fmap_entries (snapshot_map s)"
+abbreviation "snapshot_num s e \<equiv> case (snapshot_map s).[e] of Some n \<Rightarrow> Suc n | None \<Rightarrow> 0"
+definition includedIn where
+"includedIn e n snapshot \<equiv> n < snapshot_num snapshot e"
+
+instantiation snapshot :: preorder begin
+
+
+definition less_eq_snapshot  :: "snapshot \<Rightarrow> snapshot \<Rightarrow> bool"  where
+"less_eq_snapshot x y \<equiv> \<forall>(e,n)\<in>snapshot_entries x. Suc n \<le> snapshot_num y e"
+definition "less_snapshot x y \<equiv> (\<forall>(e,n)\<in>snapshot_entries x. Suc n \<le> snapshot_num y e) \<and> (\<exists>(e,n)\<in>snapshot_entries y. n \<ge> snapshot_num x e )"
+
+
+instance
+proof 
+  fix x y z :: snapshot
+  obtain x' y' z' where [simp]: "x = Snapshot x'" and [simp]: "y = Snapshot y'" and [simp]: "z = Snapshot z'"
+    by (metis snapshot.collapse)
+
+  show "(x < y) = (x \<le> y \<and> \<not> y \<le> x)"
+    apply (auto simp add: less_eq_snapshot_def less_snapshot_def  orElse_def fmap_entries_def fmlookup_dom'_iff  split: option.splits)
+    using fmdom'I apply force
+    by (metis fmdom'I not_less_eq_eq option.sel)
+
+
+  show "x \<le> x"
+    by (auto simp add: less_eq_snapshot_def fmap_entries_def orElse_def fmdom'_notI fmlookup_dom'_iff split: option.splits)
+
+  show "\<lbrakk>x \<le> y; y \<le> z\<rbrakk> \<Longrightarrow> x \<le> z"
+    apply (auto simp add: less_eq_snapshot_def fmap_entries_def orElse_def fmdom'_notI split: option.splits)
+    apply (meson fmdom'I)
+    by fastforce
+    
+qed
+
+end
+
+end
