sugar.thy
@@ -1,0 +1,25 @@
+theory sugar 
+imports Main
+begin
+
+subsection {* Syntactic sugar *}
+
+text {* Here we define some helper functions, to shorten the notation in this document. *}
+
+definition orElse (infixr "orElse" 25) where
+"x orElse y \<equiv> (case x of Some a \<Rightarrow> a | None \<Rightarrow> y)"
+
+lemma orElse_some[simp]: "(Some x orElse y) = x"
+  by (simp add: orElse_def)
+
+lemma orElse_none[simp]: "(None orElse x) = x"
+  by (simp add: orElse_def)
+
+definition compose_forward (infixl "|>" 25) where
+"x |> f \<equiv> f x"
+
+lemma "(1 |> op+ 1 |> op* 2) = (4 :: int)"
+  by eval
+
+
+end
